proving the domination properties of eliminated phinodes. The interesting cases are showing that in a reachable block b, there cannot be a phinode like   x = phi [v1,l1] [v2,l2] ... [vn ln] all vi that are from reachable li are defined in b.
If it exists, then b should dominate all reachable incoming blocks.
Therefore, the incoming blocks cannot be entry.
Moreover, b cannot be entry, since it has phinodes.

Since b is reachable, there must exist a li reachable.
We know b must dominate li.

Let consider a simple path from entry to li, then b must be on the path.

Since b isnt entry, the simple path p from entry to b isnt empty.
The p must be like
  entry ---> a pred of b -> b
here, we need the fact that preds of b cannot be entry.

Now, similarly we can show that b is also in between entry ---> a pred of b.
So, we get a contradiction, because a simple path cannot contain b more
than once.



git-svn-id: https://webdav.seas.upenn.edu/svn/sol/vol@3977 eef5ea85-cc2e-0410-bd84-0fae1f012da8

src3.0/Transforms/phielim_spec.v
@@ -1,10 +1,81 @@
 Require Import vellvm.
 Require Import primitives.
 Require Import mem2reg.
+Require Import trans_tactic.
 
 Lemma eliminate_phi_false_spec: forall f p f'
   (Helim: (f', false) = eliminate_phi f p), f = f'.
 Admitted. (* spec *)
+
+Lemma lookupBlockViaLabelFromFdef_self: forall f bv (Huniq: uniqFdef f),
+  lookupBlockViaLabelFromFdef f (getBlockLabel bv) = ret bv.
+Admitted.
+
+Ltac solve_lookupBlockViaLabelFromFdef' :=
+match goal with
+| Huniq: uniqFdef ?f |- 
+  lookupBlockViaLabelFromFdef ?f (getBlockLabel ?b) = ret ?b =>
+    eapply lookupBlockViaLabelFromFdef_self; eauto
+| _ => solve_lookupBlockViaLabelFromFdef
+end.
+
+Require Import Dipaths.
+
+Lemma non_sdom__inv: forall f l1 l2 be (Hentry: getEntryBlock f = Some be)
+  (Hnsdom: ~ strict_domination f l1 l2),
+  l1 = l2 \/ 
+  exists vl, exists al, D_walk (vertexes_fdef f) (arcs_fdef f) 
+    (index l2) (index (getBlockLabel be)) vl al /\
+    ~ In (index l1) vl.
+Admitted.
+
+Lemma wf_phi_operands__successors: forall (S : system) (M : module) (f : fdef)
+  (l0 : l) (ps0 : phinodes) (cs0 : cmds) (tmn0 : terminator) 
+  (Hwf : wf_fdef S M f) (Huniq : uniqFdef f) (value_l_list : list (value * l))
+  (id5 : id) (typ5 : typ)
+  (Hwfops : wf_phi_operands f (block_intro l0 ps0 cs0 tmn0) id5 typ5
+              value_l_list) l1
+  (Hscs: arcs_fdef f (A_ends (index l0) (index l1))),
+  exists vid1, In (value_id vid1, l1) value_l_list.
+Admitted.
+
+Require Import Kildall.
+
+Lemma blockInFdef__bound_fdef: forall f b,
+  blockInFdefB b f = true ->
+  In (getBlockLabel b) (bound_fdef f).
+Admitted.
+
+Lemma all_non_reachable__or__ex_reachable: forall f v (vls:list (value*l)),
+  (forall l0, In (v,l0) vls -> ~ reachable f l0) \/
+  exists l0, In (v,l0) vls /\ reachable f l0.
+Proof.
+  induction vls as [|[v1 l1]]. 
+    auto.
+          
+    destruct (value_dec v v1); subst.
+      destruct (reachable_dec f l1).
+        right.
+        exists l1. simpl. auto.
+
+        destruct IHvls.
+          left. simpl.
+          intros l0 Hin.
+          destruct Hin as [Hin | Hin]; auto.
+            inv Hin. auto.
+          
+          right. destruct H0 as [l0 [Hin Hreach]].
+          exists l0. simpl. auto.
+
+      destruct IHvls.
+        left. simpl.
+        intros l0 Hin.
+        destruct Hin as [Hin | Hin]; auto.
+          inv Hin. auto.
+        
+        right. destruct H as [l0 [Hin Hreach]].
+        exists l0. simpl. auto.
+Qed.
 
 Lemma eliminate_phis_false_spec: forall f' f ps0
   (Helim: (f', false) = eliminate_phis f ps0 ), f' = f.
@@ -18,6 +89,148 @@ Proof.
     apply eliminate_phi_false_spec in HeqR. subst. auto.
 Qed.
 
+Inductive selfrefl_phi (f:fdef) (b0:block): phinode -> Prop :=
+| selfrefl_phi_intro: forall pid ty vls
+    (Hinc: insnInFdefBlockB (insn_phinode (insn_phi pid ty vls)) f b0 = true)
+    (Hid: forall v1 l1, In (v1, l1) vls -> 
+            (~ reachable f l1) \/
+            exists vid1, 
+              v1 = value_id vid1 /\ 
+              lookupBlockViaIDFromFdef f vid1 = Some b0),
+    selfrefl_phi f b0 (insn_phi pid ty vls)
+.
+
+Lemma selfrelf_phi_cannot_be_in_reachable_blocks: forall (S : system)
+  (M : module) (f : fdef)(Hwf : wf_fdef S M f) (Huniq : uniqFdef f)
+  b (Hreach: isReachableFromEntry f b) p
+  (Hsefl: selfrefl_phi f b p), False.
+Proof.
+  intros.
+  inv Hsefl.
+  apply destruct_insnInFdefBlockB in Hinc.
+  destruct Hinc as [HPinB HBinF].
+  assert (Hwfp:=HBinF). 
+  destruct b as [l0 ps0 cs0 tmn0].
+  simpl in HPinB. apply InPhiNodesB_In in HPinB.
+  eapply wf_fdef__wf_phinodes in Hwfp; eauto.
+  eapply wf_phinodes__wf_phinode in Hwfp; eauto.
+  inv Hwfp.
+  assert (lookupBlockViaIDFromFdef f 
+           (getPhiNodeID (insn_phi pid ty vls)) = 
+           Some (block_intro l0 ps0 cs0 tmn0)) as Hlkup.
+    solve_lookupBlockViaIDFromFdef.
+  match goal with
+  | H6: wf_phinode _  _ _ |- _ => destruct H6 as [Hwfops Hwflist]
+  end.
+  caseEq (getEntryBlock f); 
+    try solve [intros Hentry; apply wf_fdef__non_entry in Hwf; auto; congruence].
+  intros be Hentry.
+  destruct (l_dec (getBlockLabel be) 
+                  (getBlockLabel (block_intro l0 ps0 cs0 tmn0))) as [Heq | Hneq].
+  Case "the current block is entry? no!".
+    destruct be; simpl in *; subst.
+    assert (HBinF':=Hentry).
+    apply entryBlockInFdef in HBinF'.
+    eapply blockInFdefB_uniq in HBinF; eauto.
+    destruct HBinF as [EQ1 [EQ2 EQ3]]; subst.
+    eapply wf_fdef_entryBlock_has_no_phinodes in Hentry; eauto.
+    subst; tauto.
+
+  Case "the current block isnt enty. good".
+    assert (Hentry_sdom:=Hentry).
+    eapply entry_blockStrictDominates_others in Hentry_sdom; eauto 1.
+    assert (~ In pid (getArgsIDsOfFdef f)) as Hid5notinfh.
+      solve_notin_getArgsIDs.
+    assert (forall vid vl, 
+                ~ In vid (getArgsIDsOfFdef f) ->
+                In (value_id vid,vl) vls -> 
+                reachable f vl ->
+                exists bv, exists bvl, 
+                  lookupBlockViaLabelFromFdef f vl = Some bvl /\
+                  lookupBlockViaIDFromFdef f vid = Some bv /\
+                  domination f (getBlockLabel bv) vl) as Hvid_spec.
+       intros. eapply wf_phi_operands__elim''; eauto.
+
+    (* entry cannot be l0's incoming block, 
+       otherwise l0 must sdom entry, or be entry. *)
+    assert (forall v vl, In (v,vl) vls -> vl <> getBlockLabel be)
+      as Hincoming_neq_entry.
+      admit.
+
+    (* l0 is reachable, so one of its pred must be reachable, say l1 *)
+    assert (exists v0, exists l0, In (v0, l0) vls /\ reachable f l0)
+      as Hex_reach_pred.
+      admit.
+    destruct Hex_reach_pred as [v1 [l1 [Hinlist1 Hreach1]]].
+    assert (Hinlist1':=Hinlist1).
+    apply Hid in Hinlist1'.
+    destruct Hinlist1' as [? | [vid1 [Heq Hlkup1]]]; subst; try congruence.
+    assert (Hinlist1':=Hinlist1).
+    apply Hvid_spec in Hinlist1'; try solve [auto | solve_notin_getArgsIDs].
+    destruct Hinlist1' as [bv1 [bvl1 [Hlkupbvl1 [Hlkupbv1 Hdom]]]].
+    uniq_result.
+
+    (* Get the path from entry to l1, l0 must be on the path. *)
+    unfold domination in Hdom.
+    unfold reachable in Hreach1.
+    rewrite Hentry in Hdom. 
+    rewrite Hentry in Hreach1. 
+    destruct be as [le ? ? ?].
+    destruct Hreach1 as [vl [al Hwalk]].
+    apply DWalk_to_dpath in Hwalk.
+    destruct Hwalk as [vl0 [al0 Hpath]].
+    assert (Hwalk:=Hpath).
+    apply D_path_isa_walk in Hwalk.
+    apply_clear Hdom in Hwalk.
+
+    (* split path by l0 *)
+    assert (Hpath':=Hpath).
+    apply DP_split with (x:=index l0) in Hpath'; try solve
+      [simpl in *; destruct Hwalk; subst; auto]. 
+    destruct Hpath' as [al1 [al2 [vl1 [vl2 [Hpath1 [Hpath2 [EQ1 EQ2]]]]]]]; subst.
+
+    (* in the path from entry to l0, the neigher of l0 must be the pred of l0,
+       say ly, which cannot be entry *)
+    simpl in Hneq.
+    assert (Hpath2':=Hpath2).
+    inv Hpath2; try congruence.
+
+    match goal with
+    | H4: arcs_fdef _ (A_ends _ ?y),
+      H: D_path _ _ ?y _ _ _ |- _ => 
+       rename H4 into Harc; destruct y as [ly];
+       assert (Hwalk2:=H); apply D_path_isa_walk in Hwalk2
+    end.
+    eapply wf_phi_operands__successors in Harc; eauto 1.
+    destruct Harc as [vid2 Hinlist2].
+
+    assert (reachable f ly) as Hreachy.
+      unfold reachable. fill_ctxhole. eauto.
+
+    assert (Hinlist2':=Hinlist2).
+    apply Hid in Hinlist2'; auto.
+    destruct Hinlist2' as [Hinlist2' | [vid2' [EQ1 Hlkup2']]]; try congruence.
+    inv EQ1.
+    
+    assert (~ In vid2' (getArgsIDsOfFdef f)) as Hnotargs2.
+      solve_notin_getArgsIDs.
+
+    apply Hvid_spec in Hinlist2; auto.
+    destruct Hinlist2 as [bv2 [bvl2 [Hlkupbvl2 [Hlkupbv2 Hdom2]]]].
+    uniq_result.
+
+    (* In the path from entry to ly, l0 must be there, since l0 doms ly.
+       But, a simple path cannot contain two l0. *)
+    unfold domination in Hdom2.
+    rewrite Hentry in Hdom2.
+    apply Hdom2 in Hwalk2.
+    clear - Hwalk2 Hpath2' Hneq. simpl in *.
+    apply DP_endx_ninV in Hpath2'; try congruence.
+      apply Hpath2'.
+      simpl.
+      destruct Hwalk2; subst; auto.
+Qed.
+
 (* vid = phi [vid vid ... vid] *)
 Inductive identity_phi: phinode -> Prop :=
 | identity_phi_intro: forall vid ty vls
@@ -25,13 +238,39 @@ Inductive identity_phi: phinode -> Prop :=
     identity_phi (insn_phi vid ty vls)
 .
 
+Lemma identity_phi__selfrefl_phi: forall l0 ps0 cs0 tmn0 f p
+  (HBinF: blockInFdefB (block_intro l0 ps0 cs0 tmn0) f = true)
+  (Hin: In p ps0) (Hid: identity_phi p) (Huniq: uniqFdef f),
+  selfrefl_phi f (block_intro l0 ps0 cs0 tmn0) p.
+Proof.
+  intros.
+  inv Hid.
+  apply selfrefl_phi_intro.
+    simpl.
+    bsplit; auto. solve_in_list.
+
+    intros.
+    apply Hid0 in H. subst.
+    right.
+    exists vid. 
+    split; auto.
+      apply inGetBlockIDs__lookupBlockViaIDFromFdef; auto.
+      simpl. apply getPhiNodeID_in_getPhiNodesIDs in Hin.
+      xsolve_in_list.
+Qed.
+
 Lemma identity_phi_cannot_be_in_reachable_blocks: forall S M p f
   l0 ps0 cs0 tmn0 (Hreach: reachable f l0) 
   (Hwf: wf_fdef S M f) (Huniq: uniqFdef f)
   (HBinF: blockInFdefB (block_intro l0 ps0 cs0 tmn0) f = true)
   (Hin: In p ps0) (Hid: identity_phi p),
   False. 
-Admitted. (* dom *)
+Proof.
+  intros.
+  eapply selfrelf_phi_cannot_be_in_reachable_blocks 
+    with (b:=block_intro l0 ps0 cs0 tmn0)(p:=p) in Hwf; 
+    eauto using identity_phi__selfrefl_phi.
+Qed.
 
 (* vid = phi [vid v ... vid v] *)
 Inductive assigned_phi (v:value): phinode -> Prop :=
@@ -41,12 +280,225 @@ Inductive assigned_phi (v:value): phinode -> Prop :=
     assigned_phi v (insn_phi vid ty vls)
 .
 
+Lemma assigned_phi_unreachable_vid__selfrefl_phi: forall l0 ps0 cs0 tmn0 f ty 
+  vls vid (HBinF: blockInFdefB (block_intro l0 ps0 cs0 tmn0) f = true) id0
+  (Hin: In (insn_phi id0 ty vls) ps0) (Hreach: reachable f l0)
+  (Has: assigned_phi (value_id vid) (insn_phi id0 ty vls)) (Huniq: uniqFdef f)
+  (Hnoreachvid : forall l0 : l,
+                 In (value_id vid, l0) vls -> ~ reachable f l0),
+  selfrefl_phi f (block_intro l0 ps0 cs0 tmn0) (insn_phi id0 ty vls).
+Proof.
+  intros.
+  inv Has.
+  apply selfrefl_phi_intro.
+    simpl.
+    bsplit; auto. solve_in_list.
+
+    intros v1 l1 Hin'.
+    assert (J:=Hin').
+    apply Hassign in J.
+    destruct J; subst. 
+      right.
+      exists id0.
+      split; auto.
+        apply inGetBlockIDs__lookupBlockViaIDFromFdef; auto.
+        simpl. apply getPhiNodeID_in_getPhiNodesIDs in Hin.
+        xsolve_in_list.
+
+      left. auto.
+Qed.
+
 Lemma assigned_phi__domination: forall S M p f l0 ps0 cs0 tmn0
   (Hwf: wf_fdef S M f) (Huniq: uniqFdef f)
   (HBinF: blockInFdefB (block_intro l0 ps0 cs0 tmn0) f = true) 
   (Hin: In p ps0) v (Has: assigned_phi v p),
   valueDominates f v (value_id (getPhiNodeID p)).
-Admitted. (* dom *)
+Proof.
+  intros.
+  destruct v as [vid|]; simpl; auto.
+  intros Hidreach.
+  assert (Hwfp:=HBinF).
+  eapply wf_fdef__wf_phinodes in Hwfp; eauto.
+  eapply wf_phinodes__wf_phinode in Hwfp; eauto.
+  inv Hwfp.
+  assert (lookupBlockViaIDFromFdef f 
+           (getPhiNodeID (insn_phi id5 typ5 value_l_list)) = 
+           Some (block_intro l0 ps0 cs0 tmn0)) as Hlkup.
+    solve_lookupBlockViaIDFromFdef.
+  assert (isReachableFromEntry f (block_intro l0 ps0 cs0 tmn0)) as Hreach.
+    apply Hidreach; auto.
+  match goal with
+  | H6: wf_phinode _  _ _ |- _ => destruct H6 as [Hwfops Hwflist]
+  end.
+  caseEq (getEntryBlock f); 
+    try solve [intros Hentry; apply wf_fdef__non_entry in Hwf; auto; congruence].
+  intros be Hentry.
+  destruct (l_dec (getBlockLabel be) 
+                  (getBlockLabel (block_intro l0 ps0 cs0 tmn0))) as [Heq | Hneq].
+  Case "the current block is entry? no!".
+    destruct be; simpl in *; subst.
+    assert (HBinF':=Hentry).
+    apply entryBlockInFdef in HBinF'.
+    eapply blockInFdefB_uniq in HBinF; eauto.
+    destruct HBinF as [EQ1 [EQ2 EQ3]]; subst.
+    eapply wf_fdef_entryBlock_has_no_phinodes in Hentry; eauto.
+    subst; tauto.
+
+  Case "the current block isnt enty. good".
+    assert (Hentry_sdom:=Hentry).
+    eapply entry_blockStrictDominates_others in Hentry_sdom; eauto 1.
+    unfold idDominates.
+    fill_ctxhole. 
+    caseEq (inscope_of_id f (block_intro l0 ps0 cs0 tmn0)
+       (getPhiNodeID (insn_phi id5 typ5 value_l_list))); 
+      try solve [intros Hinscope; contradict Hinscope;
+                 apply inscope_of_id__total].
+    unfold inscope_of_id, init_scope.
+    intros ids1 Hinscope.
+    destruct_if.
+    SCase "id5 in ps. nice".
+      remember (Maps.AMap.get l0 (dom_analyze f)) as R.
+      destruct R.
+      destruct (in_dec id_dec vid (getArgsIDsOfFdef f)) as [Hinfh | Hnotinfh].
+      SSCase "vid in args".
+        apply fold_left__init in H2. auto.
+ 
+      SSCase "vid notin args".
+        assert (~ In id5 (getArgsIDsOfFdef f)) as Hid5notinfh.
+          solve_notin_getArgsIDs.
+        assert (forall vid vl, 
+                ~ In vid (getArgsIDsOfFdef f) ->
+                In (value_id vid,vl) value_l_list -> 
+                reachable f vl ->
+                exists bv, exists bvl, 
+                  lookupBlockViaLabelFromFdef f vl = Some bvl /\
+                  lookupBlockViaIDFromFdef f vid = Some bv /\
+                  domination f (getBlockLabel bv) vl) as Hvid_spec.
+          intros. eapply wf_phi_operands__elim''; eauto.
+        assert ((forall l0, In (value_id vid,l0) value_l_list -> ~ reachable f l0) \/
+                 exists l0, In (value_id vid,l0) value_l_list /\ reachable f l0) as Hdec.
+          apply all_non_reachable__or__ex_reachable; auto.
+
+        destruct Hdec as [Hnoreachvid | [vl [Hinlist Hreachvid]]].
+        SSSCase "no vid is reachable".
+          eapply assigned_phi_unreachable_vid__selfrefl_phi in Has; eauto. 
+          elimtype False.
+          eapply selfrelf_phi_cannot_be_in_reachable_blocks in Has; eauto.
+
+        SSSCase "vid is reach".
+          eapply wf_phi_operands__elim' in Hinlist; eauto.
+          destruct Hinlist 
+            as [blv [Hlkupblv [[[bv [Hlkbv Hdom]]|Hnreachblv]|?]]]; 
+            try congruence.
+          SSSSCase "bv doms blv". 
+            destruct (sdom_dec f (getBlockLabel bv) l0) as [Hsdom | Hnsdom].
+            SSSSSCase "bv sdoms blv".
+              apply fold_left__spec in H2.
+              destruct H2 as [_ [H2 _]].
+              eapply H2 with (b1:=bv)(l1:=getBlockLabel bv); eauto 1.
+                assert (getBlockLabel bv <> l0) as Hneq'.
+                  destruct Hsdom; auto.
+                apply lookupBlockViaIDFromFdef__blockInFdefB in Hlkbv; auto.
+                destruct bv.
+                eapply sdom_is_complete in Hsdom; eauto 1.
+                  rewrite <- HeqR0 in Hsdom.
+                  apply ListSet.set_diff_intro; auto.
+                    simpl in *. intro J. destruct J as [J|J]; auto.
+
+                  eapply blockStrictDominates__non_empty_contents in Hentry_sdom; 
+                    eauto.
+                solve_lookupBlockViaLabelFromFdef'.
+                solve_in_list. auto.
+            SSSSSCase "bv doesnt sdom blv".
+              eapply non_sdom__inv in Hnsdom; eauto 1.
+              destruct Hnsdom as [EQ | Hnsdom]; subst.
+              SSSSSSCase "all incomings are self".
+                elimtype False.
+                eapply selfrelf_phi_cannot_be_in_reachable_blocks 
+                  with (p:=insn_phi id5 typ5 value_l_list); eauto.
+                  apply selfrefl_phi_intro.
+                    simpl. bsplit; auto. solve_in_list.
+
+                    intros v1 l1 Hinlist.
+                    inv Has.
+                    apply Hassign in Hinlist.
+                    right.
+                    destruct Hinlist; subst.
+                      exists id5.
+                      split; auto.
+                        
+                      exists vid.
+                      split; auto.
+                        assert (J:=Hlkbv).
+                        apply lookupBlockViaIDFromFdef__blockInFdefB in J.
+                        destruct bv.
+                        eapply blockInFdefB_uniq in HBinF; eauto.
+                        destruct HBinF as [EQ1 [EQ2 EQ3]]; subst. auto.
+
+              SSSSSSCase "ex a non-sdom walk".
+                destruct Hnsdom as [vl1 [al1 [Hwalk Hnotonwalk]]].
+                apply DWalk_to_dpath' in Hwalk.
+                (* consider a simple path from entry to l0, which doesnt
+                   contain vid's block *)
+                destruct Hwalk as [vl0 [al0 [Hpath Hinc]]].
+                simpl in Hneq.
+                inv Hpath; try congruence.
+                match goal with
+                | H: D_path _ _ _ _ _ _ |- _ => 
+                  assert (Hwalk:=H); apply D_path_isa_walk in Hwalk
+                end.
+                destruct y as [ly].
+                assert (reachable f ly) as Hreachy.
+                  unfold reachable. fill_ctxhole. destruct be. eauto.
+                match goal with
+                | H4: arcs_fdef _ _ |- _ => rename H4 into Harc
+                end.
+                eapply wf_phi_operands__successors in Harc; eauto 1.
+                destruct Harc as [vid1 Hinlist].
+                assert (Hvid_eq:=Hinlist).
+                inv Has.
+                apply Hassign in Hvid_eq.
+
+                (* the path must be from pid or vid's incoming blocks *)
+                destruct Hvid_eq as [Hvid_eq | Hvid_eq]; inv Hvid_eq.
+                SSSSSSSCase "from pid".
+                  (* pid must appear between entry to pred, then this is
+                     not a simple path *)
+                  eapply Hvid_spec in Hinlist; eauto 1.
+                  destruct Hinlist 
+                    as [by0 [bly0 [Hlkbly0 [Hlkby0 Hby0_dom_bly0]]]].
+                  simpl in *. uniq_result.
+                  lookupBlockViaLabelFromFdef_inv_tac.
+                  unfold domination in Hby0_dom_bly0.
+                  rewrite Hentry in Hby0_dom_bly0.
+                  destruct be as [le ? ? ?].
+                  apply Hby0_dom_bly0 in Hwalk.
+                  destruct Hwalk as [Hinpath | EQ]; subst; simpl in *; try congruence.
+                  apply H7 in Hinpath. inv Hinpath. congruence.
+
+                SSSSSSSCase "from vid".
+                  (* then vid's block must appear in the path, contradict. *)
+                  eapply Hvid_spec in Hinlist; eauto 1.
+                  destruct Hinlist 
+                    as [by0 [bly0 [Hlkbly0 [Hlkby0 Hby0_dom_bly0]]]].
+                  simpl in *. uniq_result.
+                  lookupBlockViaLabelFromFdef_inv_tac.
+                  unfold domination in Hby0_dom_bly0.
+                  rewrite Hentry in Hby0_dom_bly0.
+                  destruct be as [le ? ? ?].
+                  apply Hby0_dom_bly0 in Hwalk.
+                  contradict Hnotonwalk.
+                  destruct Hwalk as [Hinpath | EQ]; 
+                    subst; simpl in *; apply Hinc; auto.
+              
+          SSSSCase "blv is unreach".
+            lookupBlockViaLabelFromFdef_inv_tac.
+            simpl in *. congruence.
+
+    SCase "id5 notin ps? no".
+      clear HeqR.
+      contradict n. solve_in_list.
+Qed.
 
 Lemma eliminate_phi_true_spec: forall S M f b f'
   (Hreach: isReachableFromEntry f b) p 
